lam_ses_no_check.v
@@ -1,467 +1,230 @@
-Require Import Util.
-Require Import Program.
-Require Import refocusing_semantics.
-Require Import refocusing_semantics_derivation.
-Require Import abstract_machine.
-Require Import refocusing_machine.
-Require Import reduction_semantics_facts.
-Require Import lam_ses_no.
+Require Import Util
+               Entropy
+               Program
+               Subset
+               rewriting_system
+               refocusing_semantics
+               abstract_machine
+               refocusing_machine
+               reduction_languages_facts
+               lam_ses_no.
 
 
 
 
-Module Lam_SES_NO_HandSem <: RED_SEM Lam_SES_NO_Cal.RedLang.
+Module Lam_SES_NO_HandDecProc.
 
-  Module RF := RED_LANG_Facts Lam_SES_NO_RefLang.
-  Import Lam_SES_NO_RefLang.
-  Import RF.
-
-
-  Inductive dec' : term -> forall {k1 k2}, context k1 k2 -> decomp k1 -> Prop :=
-
-  | d_Var    : forall n {k1 k2} (c : context k1 k2) d, CECaD k2 ->
-                 decctx (vVar n k2) c d ->
-                 dec' (Var n) c d
-
-  | d_LamC   : forall t {k1} (c : context k1 C) d,
-                 dec' t (lam_c =: c) d -> (*!*)
-                 dec' (Lam t) c d
-  | d_LamECa : forall t {k1} (c : context k1 ECa) d,
-                 decctx (vECaLam t) c d -> (*!*)
-                 dec' (Lam t) c d
-  | d_LamD  : forall t {k1} (c : context k1 D) d,
-                 decctx (vDLam t) c d -> (*!*)
-                 dec' (Lam t) c d
-
-  | d_App    : forall t1 t2 {k1 k2} (c : context k1 k2) d, CECa k2 ->
-                 dec' t1 (ap_r t2 =: c) d ->
-                 dec' (App t1 t2) c d
-
-  | d_AppD   : forall t1 t2 {k1} (c : context k1 D) d,
-                 decctx (vDApp t1 t2) c d ->
-                 dec' (App t1 t2) c d
-
-  | d_Sub    : forall t1 n t2 {k1 k2} (c : context k1 k2) d, CECaD k2 ->
-                 dec' t1 (stag_c (n, st_sub t2) =: c) d ->
-                 dec' (Sub t1 n t2) c d
-
-  | d_Shift  : forall t1 n m {k1 k2} (c : context k1 k2) d, CECaD k2 ->
-                 dec' t1 (stag_c (n, st_shift m) =: c) d ->
-                 dec' (Shift t1 n m) c d
+  Module RF := RED_LANG_Facts Lam_SES_NO_PreRefSem.
+  Import Lam_SES_NO_PreRefSem RF.
 
 
-  with decctx : forall {k2}, value k2 -> 
-                forall {k1}, context k1 k2 -> decomp k1 -> Prop :=
+  Inductive dec_proc {k1} :  forall {k2}, term -> context k1 k2 -> decomp k1 -> Prop :=
 
-  | dc_end        : forall {k} (v : value k),
-                      ~ dead_ckind k ->
-                      decctx v [.] (d_val v)
+  | d_Var    : forall n {k2} (c : context k1 k2) d, CECaD k2 ->
+                 decctx_proc (vVar n k2) c d ->
+                 dec_proc (Var n) c d
 
-  | dc_ap_rLamC   : forall t0 t {k1} (c : context k1 C),
-                      decctx (vECaLam t0) (ap_r t =: c) (d_red (rCApp t0 t) c)
-  | dc_ap_rLamECa : forall t0 t {k1} (c : context k1 ECa),
-                      decctx (vECaLam t0) (ap_r t =: c) (d_red (rECaApp t0 t) c)
+  | d_LamC   : forall t (c : context k1 C) d,
+                 dec_proc t (lam_c =: c) d -> (*!*)
+                 dec_proc (Lam t) c d
+  | d_LamECa : forall t (c : context k1 ECa) d,
+                 decctx_proc (vECaLam t) c d -> (*!*)
+                 dec_proc (Lam t) c d
+  | d_LamD  : forall t (c : context k1 D) d,
+                 decctx_proc (vDLam t) c d -> (*!*)
+                 dec_proc (Lam t) c d
 
-  | dc_ap_rVarC   : forall n t {k1} (c : context k1 C) d,
-                      dec' t (ap_l (vCaVar n) =: c) d ->
-                      decctx (vECaVar n) (ap_r t =: c) d
-  | dc_ap_rVarECa : forall n t {k1} (c : context k1 ECa) d,
-                      dec' t (ap_l (vCaVar n) =: c) d ->
-                      decctx (vECaVar n) (ap_r t =: c) d
+  | d_App    : forall t1 t2 {k2} (c : context k1 k2) d, CECa k2 ->
+                 dec_proc t1 (ap_r t2 =: c) d ->
+                 dec_proc (App t1 t2) c d
 
-  | dc_ap_rAppC   : forall v1 v2 t {k1} (c : context k1 C) d,
-                      dec' t (ap_l (vCaApp v1 v2) =: c) d ->
-                      decctx (vECaApp v1 v2) (ap_r t =: c) d
-  | dc_ap_rAppECa : forall v1 v2 t {k1} (c : context k1 ECa) d,
-                      dec' t (ap_l (vCaApp v1 v2) =: c) d ->
-                      decctx (vECaApp v1 v2) (ap_r t =: c) d
+  | d_AppD   : forall t1 t2 (c : context k1 D) d,
+                 decctx_proc (vDApp t1 t2) c d ->
+                 dec_proc (App t1 t2) c d
 
-  | dc_ap_lC      : forall v1 v2 {k1} (c : context k1 C) d,
-                      decctx (vCApp v1 v2) c d ->
-                      decctx v2 (ap_l v1 =: c) d
-  | dc_ap_lECa    : forall v1 v2 {k1} (c : context k1 ECa) d,
-                      decctx (vECaApp v1 v2) c d ->
-                      decctx v2 (ap_l v1 =: c) d
+  | d_Sub    : forall t1 n t2 {k2} (c : context k1 k2) d, CECaD k2 ->
+                 dec_proc t1 (stag_c (n, st_sub t2) =: c) d ->
+                 dec_proc (Sub t1 n t2) c d
 
-  | dc_lam_cC     : forall v {k1} (c : context k1 C) d,
-                      decctx (vCLam v) c d ->
-                      decctx v (lam_c =: c) d
+  | d_Shift  : forall t1 n m {k2} (c : context k1 k2) d, CECaD k2 ->
+                 dec_proc t1 (stag_c (n, st_shift m) =: c) d ->
+                 dec_proc (Shift t1 n m) c d
 
-  | dc_sub_cLamC   : forall t d {k1} (c : context k1 C),
-                       decctx (vDLam t) (stag_c d =: c) (d_red (rSubLam C I t d) c)
-  | dc_sub_cLamECa : forall t d {k1} (c : context k1 ECa), 
-                       decctx (vDLam t) (stag_c d =: c) (d_red (rSubLam ECa I t d) c)
-  | dc_sub_cLamD   : forall t d {k1} (c : context k1 D), 
-                       decctx (vDLam t) (stag_c d =: c) (d_red (rSubLam D I t d) c)
 
-  | dc_sub_cVarC   : forall n d {k1} (c : context k1 C), 
-                       decctx (vDVar n) (stag_c d =: c) (d_red (rSubVar C I n d) c)
-  | dc_sub_cVarECa : forall n d {k1} (c : context k1 ECa), 
-                       decctx (vDVar n) (stag_c d =: c) (d_red (rSubVar ECa I n d) c)
-  | dc_sub_cVarD   : forall n d {k1} (c : context k1 D), 
-                       decctx (vDVar n) (stag_c d =: c) (d_red (rSubVar D I n d) c)
+  with decctx_proc {k1} : forall {k2}, value k2 -> 
+                              context k1 k2 -> decomp k1 -> Prop :=
 
-  | dc_sub_cAppC   : forall t1 t2 d {k1} (c : context k1 C), 
-                       decctx (vDApp t1 t2) (stag_c d =: c) 
+  | dc_end        : forall (v : value k1),
+                      ~ dead_ckind k1 ->
+                      decctx_proc v [.] (d_val v)
+
+  | dc_ap_rLamC   : forall t0 t (c : context k1 C),
+                      decctx_proc (vECaLam t0) (ap_r t =: c) (d_red (rCApp t0 t) c)
+  | dc_ap_rLamECa : forall t0 t (c : context k1 ECa),
+                      decctx_proc (vECaLam t0) (ap_r t =: c) (d_red (rECaApp t0 t) c)
+
+  | dc_ap_rVarC   : forall n t (c : context k1 C) d,
+                      dec_proc t (ap_l (vCaVar n) =: c) d ->
+                      decctx_proc (vECaVar n) (ap_r t =: c) d
+  | dc_ap_rVarECa : forall n t (c : context k1 ECa) d,
+                      dec_proc t (ap_l (vCaVar n) =: c) d ->
+                      decctx_proc (vECaVar n) (ap_r t =: c) d
+
+  | dc_ap_rAppC   : forall v1 v2 t (c : context k1 C) d,
+                      dec_proc t (ap_l (vCaApp v1 v2) =: c) d ->
+                      decctx_proc (vECaApp v1 v2) (ap_r t =: c) d
+  | dc_ap_rAppECa : forall v1 v2 t (c : context k1 ECa) d,
+                      dec_proc t (ap_l (vCaApp v1 v2) =: c) d ->
+                      decctx_proc (vECaApp v1 v2) (ap_r t =: c) d
+
+  | dc_ap_lC      : forall v1 v2 (c : context k1 C) d,
+                      decctx_proc (vCApp v1 v2) c d ->
+                      decctx_proc v2 (ap_l v1 =: c) d
+  | dc_ap_lECa    : forall v1 v2 (c : context k1 ECa) d,
+                      decctx_proc (vECaApp v1 v2) c d ->
+                      decctx_proc v2 (ap_l v1 =: c) d
+
+  | dc_lam_cC     : forall v (c : context k1 C) d,
+                      decctx_proc (vCLam v) c d ->
+                      decctx_proc v (lam_c =: c) d
+
+  | dc_sub_cLamC   : forall t d (c : context k1 C),
+                      decctx_proc (vDLam t) (stag_c d =: c) 
+                                  (d_red (rSubLam C I t d) c)
+  | dc_sub_cLamECa : forall t d (c : context k1 ECa),
+                      decctx_proc (vDLam t) (stag_c d =: c) 
+                                  (d_red (rSubLam ECa I t d) c)
+  | dc_sub_cLamD   : forall t d (c : context k1 D),
+                      decctx_proc (vDLam t) (stag_c d =: c)
+                                  (d_red (rSubLam D I t d) c)
+
+  | dc_sub_cVarC   : forall n d (c : context k1 C),
+                      decctx_proc (vDVar n) (stag_c d =: c) 
+                                  (d_red (rSubVar C I n d) c)
+  | dc_sub_cVarECa : forall n d (c : context k1 ECa),
+                      decctx_proc (vDVar n) (stag_c d =: c) 
+                                  (d_red (rSubVar ECa I n d) c)
+  | dc_sub_cVarD   : forall n d (c : context k1 D),
+                      decctx_proc (vDVar n) (stag_c d =: c) 
+                                  (d_red (rSubVar D I n d) c)
+
+  | dc_sub_cAppC   : forall t1 t2 d (c : context k1 C),
+                      decctx_proc (vDApp t1 t2) (stag_c d =: c)
                                   (d_red (rSubApp C I t1 t2 d) c)
-  | dc_sub_cAppECa : forall t1 t2 d {k1} (c : context k1 ECa), 
-                       decctx (vDApp t1 t2) (stag_c d =: c) 
+  | dc_sub_cAppECa : forall t1 t2 d (c : context k1 ECa),
+                      decctx_proc (vDApp t1 t2) (stag_c d =: c) 
                                   (d_red (rSubApp ECa I t1 t2 d) c)
-  | dc_sub_cAppD   : forall t1 t2 d {k1} (c : context k1 D), 
-                       decctx (vDApp t1 t2) (stag_c d =: c) 
+  | dc_sub_cAppD   : forall t1 t2 d (c : context k1 D),
+                      decctx_proc (vDApp t1 t2) (stag_c d =: c) 
                                   (d_red (rSubApp D I t1 t2 d) c).
 
-  Definition dec := dec'. Arguments dec t {k1 k2} c d.
-
-  Scheme dec_Ind    := Induction for dec' Sort Prop
-    with decctx_Ind := Induction for decctx Sort Prop.
+  Scheme dec_proc_Ind    := Induction for dec_proc Sort Prop
+    with decctx_proc_Ind := Induction for decctx_proc Sort Prop.
 
 
-  (* Non-signature entries (helpers): *)
-
-  Lemma dead_dec_dead : 
-      forall {k1} (c : context k1 CBot) v d, ~ dec v c d.
-
-  Proof with autof.
-    intros; intro H.
-    dependent destruction H...
-  Qed.
-
-
-  Lemma dead_decctx_dead : 
-      forall {k1} (c : context k1 CBot) v d, ~ decctx v c d.
-
-  Proof with autof.
-    intros; intro H.
-    dependent destruction H...
-  Qed.
-
-
-  Ltac inj_vr := 
-      match goal with
-      | [Hv : value_to_term _ = value_to_term _ |- _] => 
-            apply value_to_term_injective in Hv
-      | [Hv : valCa_to_term _ = valCa_to_term _ |- _] => 
-            apply valCa_to_term_injective in Hv
-      | [Hr : redex_to_term _ = redex_to_term _ |- _] => 
-            apply redex_to_term_injective in Hr
-      | [ |- _] => idtac
-      end.
-
-
-  Lemma dec_val_self : forall {k2} (v : value k2) {k1} (c : context k1 k2) d, 
-                           dec (v : term) c d <-> decctx v c d.
-
-  Proof with auto.
-    induction v using val_Ind with
-    (P := fun k2 (v : value k2) => forall (k1 : ckind) (c : context k1 k2)
-              (d : decomp k1), dec (v : term) c d <-> decctx v c d)
-    (P0:= fun v0 : valCa => forall (k1 k2 : ckind) (c : context k1 k2) (v : value k2)
-              (d : decomp k1), (valCa_to_term v0 : term) = (v : term) -> 
-              (dec (v : term) c d <-> decctx v c d));
-
-    intros;
-    try match goal with [ H: (valCa_to_term ?v0) = (value_to_term ?v1) |- _ ] => 
-        match type of v0 with valCa => 
-            destruct v1; autof; 
-            inversion H; repeat inj_vr; subst; 
-            clear H
-        end
-    end;
-
-    split; intro H1;
-
-    dependent destruction H1;
-    try solve
-    (* Cases of: dec v c d -> decctx v c d. *)
-    [ rewrite IHv in H1;
-      dependent destruction H1;
-      auto
-    | match goal with v : valCa |- _ =>
-      destruct valCa_is_valECa with v as (v', H2);
-      destruct v; dependent destruction v'; autof;
-      inversion H2; repeat inj_vr; subst;
-      rewrite H2 in H1;
-      rewrite IHv in H1; auto;
-      dependent destruction H1;
-      match goal with v0 : val _ |- _ => match goal with H : dec' (_ v0) _ _ |- _ =>
-      rewrite IHv0 in H;
-      dependent_destruction2 H;
-      auto
-      end end end 
-    | match goal with H : dec' _ _ _ |- _ =>
-      contradiction (dead_dec_dead _ _ _ H)
-      end
-    | match goal with H : Var _ = _ |- _ => 
-      dependent destruction v; 
-      inversion H; subst; 
-      simpl in *; tauto 
-      end
-
-    (* Cases of: dec v c d <- decctx v c d. *)
-    | first [apply d_AppD | constructor]; (* imaginary fold *)
-      try (rewrite IHv; constructor); 
-      constructor; 
-      auto
-    | match goal with v : valCa |- _ =>
-      constructor; simpl; auto; (* imaginary fold *) fold valCa_to_term;
-      destruct valCa_is_valECa with v as (v', H2);
-      destruct v; dependent destruction v'; autof;
-      inversion H2; repeat inj_vr; subst;
-      rewrite H2;
-      rewrite IHv; auto; constructor;
-      rewrite IHv0; constructor;
-      constructor;
-      auto
-      end
-
-    (* Cases of both implications. *)
-    | autof ].
-  Qed.
-
-
-
-  (* Signature entries: *)
-
-  Lemma dec_correct : forall {t k1 k2} {c : context k1 k2} {d}, 
-                          dec t c d -> c[t] = d.
-  Proof with auto.
-    induction 1 using dec_Ind with
-    (P  := fun t _ _ c d (_ : dec t c d)    => c[t] = d)
-    (P0 := fun _ v _ c d (_ : decctx v c d) => c[v] = d)...
-    
-    - destruct k2...
-  Qed.
-
-
-  Lemma dec_plug :
-      forall {k1 k2} (c : context k1 k2) {k3} {c0 : context k3 k1} {t d}, 
-          ~ dead_ckind k2 -> dec c[t] c0 d -> dec t (c ~+ c0) d.
-  Proof.
-    intros k1 k2.
-    induction c.
-    - auto.
-    - intros k3 c0 t0 d H H0.
-      destruct ec0;
-          destruct_all sub_tag; destruct_all substitut;
-          assert (hh := IHc _ _ _ _ (death_propagation2 _ _ H) H0);
-          dependent destruction hh; subst;
-          try destruct k2; autof;
-      solve
-      [ autof
-      | destruct valCa_is_valECa with v as (v', H2);
-        destruct v; dependent destruction v'; 
-        solve
-        [ autof
-        | inversion H2; repeat inj_vr; subst;
-          rewrite H2 in hh;
-          rewrite dec_val_self in hh;
-          dependent destruction hh;
-          auto 
-      ] ].
-  Qed.
-
-
-  Lemma dec_plug_rev :
-      forall {k1 k2} (c : context k1 k2) {k3} {c0 : context k3 k1} {t d}, 
-          ~ dead_ckind k2 -> dec t (c ~+ c0) d -> dec c[t] c0 d.
-  Proof.
-    induction c.
-    - auto.
-    - intros k3 c0 t d H H0.
-      simpl.
-      apply IHc; eauto using death_propagation2.
-      destruct ec0, k2;
-      destruct_all sub_tag; destruct_all substitut;
-      try solve 
-      [ autof 
-      | constructor; simpl; auto
-      | match goal with v : valCa |- _ =>
-        destruct (valCa_is_valECa v) as (v', H1);
-        destruct v; dependent destruction v'; 
-        inversion H1; repeat inj_vr; subst;
-        constructor; try solve [simpl; auto];
-        rewrite H1;
-        apply dec_val_self;
-        constructor;
-        assumption
-        end ].
-  Qed.
-
-
-  Lemma dec_redex_self : forall {k2} (r : redex k2) {k1} (c : context k1 k2), 
-                             dec (redex_to_term r) c (d_red r c).
-  Proof with auto.
-    destruct r as [t1 t2 | t1 t2 | k H n d | k H t d | k H t1 t2 d];
-    destruct_all sub_tag; destruct_all substitut;
-    try solve
-    [ intros;
-      constructor; try solve [simpl; auto];
-      first 
-      [ destruct k; destruct H; first [apply d_AppD | constructor]; simpl; autof
-      | rewrite (dec_val_self (vECaLam t1)) ];
-      constructor ].
-  Qed.
-
-
-  Lemma dec_value_self : forall {k} (v : value k), 
-                             ~ dead_ckind k -> dec v [.] (d_val v).
-  Proof with auto.
-    intros k v H.
-    apply dec_val_self.
-    constructor...
-  Qed.
-
-
-  Inductive decempty : term -> forall {k}, decomp k -> Prop :=
-  | d_intro : forall {t k} {d : decomp k}, dec t [.] d -> decempty t d.
-
-  Inductive iter : forall {k}, decomp k -> value k -> Prop :=
-  | i_val : forall {k} (v : value k), iter (d_val v) v
-  | i_red : forall {k2} (r : redex k2) {t k1} (c : context k1 k2) {d v},
-                contract r = Some t -> decempty c[t] d -> iter d v ->
-                iter (d_red r c) v.
-
-  Inductive eval : term -> value init_ckind -> Prop :=
-  | e_intro : forall {t} {d : decomp init_ckind} {v : value init_ckind}, 
-                  decempty t d -> iter d v -> eval t v.
-
-End Lam_SES_NO_HandSem.
-
-
-
-
-Module Lam_SES_NO_RefSem_Check.
-
-  Import Lam_SES_NO_RefLang Lam_SES_NO_Strategy.
-
-  Module HS := Lam_SES_NO_HandSem.
   Module RS := Lam_SES_NO_RefSem.
 
 
-  Lemma HS_dec_imp_RS_dec : 
-      forall t {k1 k2} (c : context k1 k2) d, HS.dec t c d -> RS.dec t c d.
+  Hint Constructors RS.dec_proc RS.decctx_proc dec_proc decctx_proc.
+  Hint Transparent Lam_SES_NO_Strategy.dec_term Lam_SES_NO_Strategy.dec_context.
+
+  Theorem dec_proc_eqv_RS :                       forall {k1 k2} (c : context k1 k2) t d,
+      dec_proc t c d <-> RS.dec_proc t c d.
 
   Proof.
-    induction 1 using HS.dec_Ind with
-    (P := fun t _ _ c d (_ : HS.dec t c d)    =>  RS.dec t c d)
-    (P0:= fun _ v _ c d (_ : HS.decctx v c d) =>  RS.decctx v c d);
-    try destruct k2; autof;
-    try solve
-    [ econstructor; simpl; eauto (* - sementicaly this is enough, but Ltac is 
-                                      too weak, so we need to be more explicite *)
-    | eapply @RS.d_term; simpl; eauto 
-    | eapply @RS.dc_dec  with (ec:=ap_r _)   (k2:= C);   simpl; auto
-    | eapply @RS.dc_term with (ec:=ap_r _)   (k2:= C);   simpl; eauto 
-    | eapply @RS.dc_dec  with (ec:=ap_r _)   (k2:= ECa); simpl; auto
-    | eapply @RS.dc_term with (ec:=ap_r _)   (k2:= ECa); simpl; eauto
-    | eapply @RS.dc_val  with (ec:=ap_l _)   (k2:= C);   simpl; auto
-    | eapply @RS.dc_val  with (ec:=ap_l _)   (k2:= ECa); simpl; auto
-    | eapply @RS.dc_val  with (ec:=lam_c)    (k2:= C);   simpl; auto
-    | eapply @RS.dc_dec  with (ec:=stag_c _) (k2:= C);   simpl; auto
-    | eapply @RS.dc_dec  with (ec:=stag_c _) (k2:= ECa); simpl; auto
-    | eapply @RS.dc_dec  with (ec:=stag_c _) (k2:= D);   simpl; auto ].
-  Qed.
- 
+    intros k1 k2 c t d; split; intro H.
 
-  Lemma RS_dec_imp_HS_dec : 
-      forall t {k1 k2} (c : context k1 k2) d, RS.dec t c d -> HS.dec t c d.
-
-  Proof.
-    induction 1 using RS.dec_Ind with
-    (P := fun t _ _ c d (_ : RS.dec t c d)    => HS.dec t c d)
-    (P0:= fun _ v _ c d (_ : RS.decctx v c d) => HS.decctx v c d);
-    try solve 
-    [ match goal with H : dec_term _ _ = _ |- _ =>
-      destruct t, k2; 
-      inversion H; subst; 
-      first [apply HS.d_AppD | constructor]; simpl; auto
-      end
-    | match goal with H : dec_context _ _ _ = _ |- _ =>
-      destruct ec0, k2; dependent destruction v; 
-      inversion H; subst; 
-      constructor; auto
-      end 
-    | constructor; auto ].
-  Qed.
-
-
-  Lemma dec_eqv : 
-      forall t {k1 k2} (c : context k1 k2) d, HS.dec t c d <-> RS.dec t c d.
-
-  Proof.
-    split;
-    solve[ eauto using RS_dec_imp_HS_dec, HS_dec_imp_RS_dec ].
-  Qed.
-
-
-  Lemma decempty_eqv : 
-      forall t {k} (d : decomp k), HS.decempty t d <-> RS.decempty t d.
-
-  Proof with auto.
-    split; 
-
-    solve
-    [ intro H;
-      dependent_destruction2 H;
-      constructor;
-      apply dec_eqv; auto ].
-  Qed.
-
-
-  Lemma iter_eqv : forall {k} (d : decomp k) v, 
-                           HS.iter d v <-> RS.iter d v.
-  Proof.
-    split;
- 
-    solve
-    [ intro H;
-      dependent induction H;
+  (* -> *) { 
+    induction H using dec_proc_Ind with
+    (P0 := fun _ v c d _ => RS.decctx_proc v c d); 
+    solve 
+    [ try destruct k2; eautof
+    | match goal with c : RS.context _ ?k |- RS.decctx_proc _ (?ec =: c) _ => 
       solve
-      [ constructor
-      | econstructor; 
-        solve 
-        [ eauto
-        | eapply decempty_eqv; eauto
-    ] ] ].
+      [ eapply (RS.dc_dec ec c); eauto
+      | eapply (RS.dc_val ec c); eauto
+      | eapply (RS.dc_term ec c); eauto ]
+      end ].
+  }
+
+  (* <- *) {
+    induction H using RS.dec_proc_Ind with
+    (P0 := fun _ v c d _ => decctx_proc v c d);
+    try match goal with
+    | H : RS.ST.dec_term ?t ?k = _        |- _ => destruct t, k; 
+                                                  inversion H; subst
+    | H : RS.ST.dec_context ?ec ?k ?v = _ |- _ => destruct ec, k; 
+                                                  dependent_destruction2 v; 
+                                                  inversion H; subst
+    end; eautof.
+  }
   Qed.
 
 
-  Theorem eval_eqv : 
-      forall t v, HS.eval t v <-> RS.eval t v.
+  Theorem decctx_proc_eqv_RS :                    forall {k1 k2} (c : context k1 k2) v d,
+      decctx_proc v c d <-> RS.decctx_proc v c d.
 
-  Proof with auto.
-    split;
+  Proof.
+    intros k1 k2 c v d; split; intro H.
 
-    solve
-    [ intro H;
-      dependent destruction H;
-      econstructor;
-      [ apply decempty_eqv; eauto
-      | apply iter_eqv; eauto
-    ] ].
+  (* -> *) {
+    induction H using decctx_proc_Ind with
+    (P := fun _ t c d _ => RS.dec_proc t c d); 
+    solve 
+    [ try destruct k2; eautof
+    | match goal with c : RS.context _ ?k |- RS.decctx_proc _ (?ec =: c) _ => 
+      solve
+      [ eapply (RS.dc_dec ec c); eauto
+      | eapply (RS.dc_val ec c); eauto
+      | eapply (RS.dc_term ec c); eauto ]
+      end ].
+  }
+
+  (* <- *) {
+    induction H using RS.decctx_proc_Ind with
+    (P := fun _ t c d _ => dec_proc t c d);
+    try match goal with
+    | H : RS.ST.dec_term ?t ?k = _        |- _ => destruct t, k; 
+                                                  inversion H; subst
+    | H : RS.ST.dec_context ?ec ?k ?v = _ |- _ => destruct ec, k; 
+                                                  dependent_destruction2 v; 
+                                                  inversion H; subst
+    end; 
+    solve [eauto].
+  }
   Qed.
 
-End Lam_SES_NO_RefSem_Check.
+End Lam_SES_NO_HandDecProc.
+
 
 
 
 
 Module Lam_SES_NO_HandMachine <: ABSTRACT_MACHINE.
 
-  Import Lam_SES_NO_EAM.
-  Import Lam_SES_NO_RefLang.
+  Import Lam_SES_NO_EAM Lam_SES_NO_PreRefSem.
+
+
+  Definition term          := term.
+  Definition value         := value init_ckind.
+  Definition configuration := configuration.
+  Definition load          := load.
+  Definition value_to_conf := value_to_conf.
+  Definition final         := final.
+
 
   Definition contextD := (context C C + context C ECa + context C D) %type.
   Definition contextC := (context C C + context C ECa) %type.
   Definition contextA := context C C.
 
-  Notation "[$ t $]"       := (c_eval t  [.])    (t at level 99).
-  Notation "[: v :]"       := (c_apply [.] v)    (v at level 99).
-  Notation "[$ t , c $]"   := (c_eval t c)       (t, c at level 99).
-  Notation "[: c , v :]"   := (c_apply c v)      (c, v at level 99).
-
-  Reserved Notation "c1 → c2" (at level 40).
+  Notation "[$ t $]"       := (submember_by _ (c_eval t [.]) init_ckind_alive
+                                   : configuration)                      (t at level 99).
+  Notation "[: v :]"       := (submember_by _ (c_apply [.] v) init_ckind_alive
+                                   : configuration)                      (v at level 99).
+  Notation "[$ t , k , c , H $]" := (@c_eval t k c ?& H)              (t, c at level 99).
+  Notation "[: c , v , H :]"     := (c_apply c v ?& H)                (c, v at level 99).
+  Notation "[: ( ec , k ) =: c , v , H :]" := 
+      (c_apply (@ccons _ ec k c) v ?& H)                       (ec, k, c, v at level 99).
 
 
   Lemma pre_sub_CECaD_is_CECaD : forall k d, CECaD (k+>stag_c d) -> CECaD k.
@@ -481,198 +244,135 @@ Module Lam_SES_NO_HandMachine <: ABSTRACT_MACHINE.
       end.
 
 
-  Inductive trans : configuration -> configuration -> Prop :=
+  Definition next_conf0 (st : configuration) : option configuration :=
+      match st with
 
-  (* refocus *)
+      | [$ _, CBot, _, _ $]    => None
 
-  | t_evVar      : forall n {k1 k2} (c : context k1 k2), CECaD k2 ->
-                    [$ Var n, c $]     → [: c, vVar n k2 :]
+      | [$ Var n, k, c, _ $]   => Some [: c, vVar n k, I :]
 
-  | t_evLamD     : forall t {k1} (c : context k1 D),
-                    [$ Lam t, c $] → [: c, vDLam t :]
+      | [$ Lam t, D,   c, _ $] => Some [: c, vDLam t, I :]
+      | [$ Lam t, ECa, c, _ $] => Some [: c, vECaLam t, I :]
+      | [$ Lam t, C,   c, _ $] => Some [$ t, C, lam_c =: c, I $]
 
-  | t_evLamECa : forall t {k1} (c : context k1 ECa),
-                    [$ Lam t, c $] → [: c, vECaLam t :]
+      | [$ App t1 t2, D,   c, _ $]  => Some [: c, vDApp t1 t2, I :]
+      | [$ App t1 t2, ECa, c, _ $]  => Some [$ t1, ECa, ap_r t2 =: c, I  $]
+      | [$ App t1 t2, C,   c, _ $]  => Some [$ t1, ECa, ap_r t2 =: c, I  $]
 
-  | t_evLamC     : forall t {k1} (c : context k1 C),
-                    [$ Lam t, c $] → [$ t, lam_c =: c $]
-
-  | t_evAppD   : forall t1 t2 {k1} (c : context k1 D),
-                    [$ App t1 t2, c $] → [: c, vDApp t1 t2 :]
-
-  | t_evAppECa   : forall t1 t2 {k1} (c : context k1 ECa),
-                    [$ App t1 t2, c $] → [$ t1, ap_r t2 =: c $]
-  | t_evAppC     : forall t1 t2 {k1} (c : context k1 C),
-                    [$ App t1 t2, c $] → [$ t1, ap_r t2 =: c $]
-
-  | t_evSub      : forall t1 j t2 {k1 k2} (c : context k1 k2), CECaD k2 ->
-                    [$ Sub t1 j t2, c $]  → [$ t1, stag_c (j, st_sub t2) =: c $]
-
-  | t_evShift    : forall t1 j g {k1 k2} (c : context k1 k2), CECaD k2 ->
-                    [$ Shift t1 j g, c $] → [$ t1, stag_c (j, st_shift g) =: c $]
+      | [$ Sub t1 j t2,  k, c, _ $] => Some [$ t1, _, stag_c (j, st_sub t2) =: c, I  $]
+      | [$ Shift t1 j g, k, c, _ $] => Some [$ t1, _, stag_c (j, st_shift g) =: c, I  $]
 
 
-  (* aux_D *)
+      | [: (_, CBot) =: _, _, _ :] => None
 
-  | t_apSubAppD  : forall t1 t2 {k1} (c : context k1 D) d,
-                    [: stag_c d =: c, vDApp t1 t2 :] → [$ contract0 (rSubApp D I t1 t2 d), c $]
-  | t_apSubAppECa: forall t1 t2 {k1} (c : context k1 ECa) d,
-                    [: stag_c d =: c, vDApp t1 t2 :] → [$ contract0 (rSubApp D I t1 t2 d), c $]
-  | t_apSubAppC  : forall t1 t2 {k1} (c : context k1 C) d,
-                    [: stag_c d =: c, vDApp t1 t2 :] → [$ contract0 (rSubApp D I t1 t2 d), c $]
+       (* aux_D *)
 
-  | t_apSubLamD  : forall t {k1} (c : context k1 D) d,
-                    [: stag_c d =: c, vDLam t :] → [$ contract0 (rSubLam D I t d), c $]
-  | t_apSubLamECa: forall t {k1} (c : context k1 ECa) d,
-                    [: stag_c d =: c, vDLam t :] → [$ contract0 (rSubLam D I t d), c $]
-  | t_apSubLamC  : forall t {k1} (c : context k1 C) d,
-                    [: stag_c d =: c, vDLam t :] → [$ contract0 (rSubLam D I t d), c $]
+       | [: stag_c d =: c, vDApp t1 t2, _ :] => 
+                                      Some [$ contract0 (rSubApp D I t1 t2 d), _, c, I $]
 
-  | t_apSubVarD  : forall i {k1} (c : context k1 D) d,
-                    [: stag_c d =: c, vDVar i :] → [$ contract0 (rSubVar D I i d), c $]
-  | t_apSubVarECa: forall i {k1} (c : context k1 ECa) d,
-                    [: stag_c d =: c, vDVar i :] → [$ contract0 (rSubVar D I i d), c $]
-  | t_apSubVarC  : forall i {k1} (c : context k1 C) d,
-                    [: stag_c d =: c, vDVar i :] → [$ contract0 (rSubVar D I i d), c $]
+       | [: stag_c d =: c, vDLam t, _ :] => 
+                                      Some [$ contract0 (rSubLam D I t d) , _ , c , I $]
 
-  (* aux_C *)
+       | [: stag_c d =: c, vDVar i, _ :] => 
+                                      Some [$ contract0 (rSubVar D I i d), _, c, I $]
 
-  | t_apAp_rVarECa : forall i {k1} (c : context k1 ECa) t2, 
-                       [: ap_r t2 =: c, vECaVar i :] → [$ t2, ap_l (vCaVar i) =: c $]
-  | t_apAp_rVarC   : forall i {k1} (c : context k1 C) t2, 
-                       [: ap_r t2 =: c, vECaVar i :] → [$ t2, ap_l (vCaVar i) =: c $]
+       (* aux_C *)
 
-  | t_apAp_rAppECa : forall v1 v2 {k1} (c : context k1 ECa) t2, 
-                       [: ap_r t2 =: c, vECaApp v1 v2 :] → [$ t2, ap_l (vCaApp v1 v2) =: c $]
-  | t_apAp_rAppC   : forall v1 v2 {k1} (c : context k1 C) t2, 
-                       [: ap_r t2 =: c, vECaApp v1 v2 :] → [$ t2, ap_l (vCaApp v1 v2) =: c $]
+       | [: (ap_r t2, ECa) =: c, vECaVar i, _ :] => 
+                                      Some [$ t2, C, ap_l (vCaVar i) =: c, I $]
+       | [: (ap_r t2, C)   =: c, vECaVar i, _ :] => 
+                                      Some [$ t2, C, ap_l (vCaVar i) =: c, I $]
 
-  | t_apAp_rLamECa : forall t1 {k1} (c : context k1 ECa) t2, 
-                       [: ap_r t2 =: c, vECaLam t1 :] → [$ contract0 (rECaApp t1 t2), c $]
-  | t_apAp_rLamC   : forall t1 {k1} (c : context k1 C) t2, 
-                       [: ap_r t2 =: c, vECaLam t1 :] → [$ contract0 (rECaApp t1 t2), c $]
+       | [: (ap_r t2, ECa) =: c, vECaApp v1 v2, _ :] => 
+                                      Some [$ t2, C, ap_l (vCaApp v1 v2) =: c, I $]
+       | [: (ap_r t2, C)   =: c, vECaApp v1 v2, _ :] => 
+                                      Some [$ t2, C, ap_l (vCaApp v1 v2) =: c, I $]
 
-  (* aux_A *)
+       | [: (ap_r t2, ECa) =: c, vECaLam t1, _ :] => 
+                                      Some [$ contract0 (rECaApp t1 t2), ECa, c, I $]
+       | [: (ap_r t2, C)   =: c, vECaLam t1, _ :] => 
+                                      Some [$ contract0 (rECaApp t1 t2), C, c, I $]
 
-  | t_apAp_lECa    : forall (v2 : value C) {k1} (c : context k1 ECa) v1,
-                       [: ap_l v1 =: c, v2 :] → [: c, vECaApp v1 v2 :]
-  | t_apAp_lC      : forall (v2 : value C) {k1} (c : context k1 C) v1,
-                       [: ap_l v1 =: c, v2 :] → [: c, vCApp v1 v2 :]
+       (* aux_A *)
 
-  | t_apLam_cC     : forall (v : value C) {k1} (c : context k1 C), 
-                       [: lam_c =: c, v :] → [: c, vCLam v :]
+       | [: (ap_l v1, ECa) =: c, v2, _ :] => Some [: c, vECaApp v1 v2, I :]
+       | [: (ap_l v1, C)   =: c, v2, _ :] => Some [: c, vCApp v1 v2, I :]
 
-  where "c1 → c2" := (trans c1 c2).
-  Definition transition := trans.
+       | [: (lam_c, C)     =: c, v, _ :]  => Some [: c, vCLam v, I :]
+
+       | _ => None
+       end. 
+
+  Definition next_conf (_ : entropy) := next_conf0.
+
+  Definition transition st1 st2 := next_conf0 st1 = Some st2.
 
 
-  Lemma final_correct : forall v st, ~ c_final v → st.
-  Proof. inversion 1. Qed.
+  Instance rws : REWRITING_SYSTEM configuration :=
+  { transition := transition }.
 
 
-  Reserved Notation "c1 →+ c2" (at level 40, no associativity).
+  Fact trans_computable0 :                              forall (st1 st2 : configuration),
+       `(rws) st1 → st2 <-> next_conf0 st1 = Some st2.
 
-  Inductive trans_close : configuration -> configuration -> Prop :=
-  | one_step   : forall {c0 c1 : configuration}, 
-                   c0 → c1 -> trans_close c0 c1
-  | multi_step : forall {c0 c1 c2 : configuration}, 
-                   c0 → c1 -> trans_close c1 c2 -> trans_close c0 c2
-  where "c1 →+ c2" := (trans_close c1 c2).
+  Proof. intuition. Qed.
 
 
-  Definition trans_ref_close c1 c2 := c1 = c2 \/ trans_close c1 c2.
-  Notation "c1 →* c2" := (trans_ref_close c1 c2).
+  Fact trans_computable :                                                 forall st1 st2,
+       `(rws) st1 → st2 <-> exists e, next_conf e st1 = Some st2.
 
-  Inductive eval : term -> value init_ckind -> Prop :=
-  | e_intro : forall t (v : val init_ckind), trans_close (c_init t) (c_final v) -> eval t v.
+  Proof. 
+   intuition. 
+   - destruct (draw_fin_correct 1 Fin.F1) as [e _]; exists e; auto.
+   - destruct H; eauto.
+  Qed.
 
 
-  Definition term          := term.
-  Definition value         := value init_ckind.
-  Definition configuration := configuration.
-  Definition c_init        := c_init.
-  Definition c_final       := c_final.
+
+
+  Theorem next_conf0_eq_EAM :                                                  forall st,
+      next_conf0 st = Lam_SES_NO_EAM.next_conf0 st.
+
+  Proof.
+    destruct st as [[t k ? | k c v] ?].
+    - destruct t, k; eauto.
+    - destruct c as [| ec k c]; eauto.
+      destruct ec, k; dependent destruction v; eauto.
+  Qed.
+
+
+  Corollary next_conf_eq_EAM :                                               forall e st,
+      next_conf e st = Lam_SES_NO_EAM.next_conf e st.
+
+  Proof. eauto using next_conf0_eq_EAM. Qed.
+
+
+  Corollary transition_eqv_EAM :                                          forall st1 st2,
+      `(Lam_SES_NO_EAM.rws) st1 → st2  <->  `(rws) st1 → st2.
+
+  Proof.
+    intros.
+    rewrite trans_computable, Lam_SES_NO_EAM.trans_computable.
+    unfold Lam_SES_NO_EAM.next_conf, next_conf.
+    rewrite next_conf0_eq_EAM.
+    intuition.
+  Qed.
+
+
+  Proposition final_correct :                                                  forall st,
+       final st <> None -> ~exists st', `(rws) st → st'.
+
+  Proof.
+    destruct st as [[? | ? c v] ?]; auto.
+    destruct c; auto.
+    intros _ [st' H].
+    inversion H.
+  Qed.
+
+
+  Fact finals_are_vals :                                                     forall st v,
+       final st = Some v <-> st = v. 
+
+  Proof. exact Lam_SES_NO_EAM.finals_are_vals. Qed.
 
 End Lam_SES_NO_HandMachine.
-
-
-
-
-Module Lam_SES_NO_Machine_Check.
-
-  Module EAM := Lam_SES_NO_EAM.
-  Module HM  := Lam_SES_NO_HandMachine.
-  Import EAM HM.
-  Import Lam_SES_NO_RefLang Lam_SES_NO_Strategy.
-
-
-  Notation "c1 >> c2"  := (Lam_SES_NO_EAM.transition c1 c2)  
-               (at level 40, no associativity).
-  Notation "c1 >>+ c2" := (Lam_SES_NO_EAM.trans_close c1 c2) 
-               (at level 40, no associativity).
-
-
-
-  Lemma trans_EAM2HM : forall c0 c1,  c0 >> c1  ->  c0 → c1.
-  Proof.
-    inversion 1; subst;
-    capture_all ckind term context value redex @contract;
-    capture_all dec_term dec_context @in_red @in_val @in_term;
-    match goal with
-    | H : dec_term ?t ?k2 = _ |- _        => destruct t, k2; 
-                                             inversion H; subst
-    | H : dec_context ?ec ?k2 ?v = _ |- _ => destruct ec, k2; dependent_destruction2 v; 
-                                             inversion H; subst
-    end;
-    try match goal with
-    | H : contract _ = Some _ |- _ => inversion H
-    end;
-
-    solve [ constructor; simpl; auto ].
-  Qed.
-
-
-  Lemma trans_HM2EAM : forall c0 c1,  c0 → c1  ->  c0 >> c1.
-  Proof with auto.
-    inversion 1; subst;
-    try match goal with
-    | H : CECaD ?k |- _ => destruct k; inversion H
-    | H : CECaD ?k |- _ => destruct k; inversion H
-    end;
-    solve [ econstructor; simpl; auto ].
-  Qed.
-
-
-  Lemma trans_eqv : forall c0 c1,  c0 → c1  <->  c0 >> c1.
-  Proof.
-    split; 
-    solve [ auto using trans_HM2EAM, trans_EAM2HM ].
-  Qed.
-
-
-  Lemma tramsCl_eqv : forall c0 c1,  c0 →+ c1  <->  c0 >>+ c1.
-  Proof.
-    split;
-
-    solve
-    [ intro H;
-      induction H;
-      [ constructor 1;  apply trans_eqv; auto
-      | econstructor 2; solve [eauto | apply trans_eqv; eauto]
-    ] ].
-  Qed.
-
-
-  Theorem eval_eqv : forall t v, HM.eval t v <-> EAM.eval t v.
-  Proof.
-    split;
-    
-    solve
-    [ intro H;
-      destruct H;
-      constructor;
-      apply tramsCl_eqv; auto ].
-  Qed.
-
-
-End Lam_SES_NO_Machine_Check.
